common/Memtype.v
@@ -159,7 +159,7 @@ values as prescribed by [f].  (See module [Values].)
 Likewise, a memory injection [f] defines a relation between memory states
 that we now axiomatize. *)
 
- inject: forall {injperm: InjectPerm}, meminj -> mem -> mem -> Prop;
+ inject: forall {injperm: InjectPerm}, meminj -> frameinj -> mem -> mem -> Prop;
 
 (** Memory states that inject into themselves. *)
 
@@ -179,11 +179,10 @@ that we now axiomatize. *)
 
  (* Stack ADT and methods *)
  stack_adt: mem -> list frame_adt;
- record_stack_blocks: mem -> frame_adt -> option mem;
+ record_stack_blocks: mem -> frame_adt -> mem -> Prop;
  unrecord_stack_block: mem -> option mem;
  frame_inject {injperm: InjectPerm} f m := frame_inject' f (perm m);
  stack_limit: Z;
-                                                         
 }.
 
 
@@ -1105,112 +1104,112 @@ Class MemoryModel mem `{memory_model_ops: MemoryModelOps mem}
 
 (** ** Properties of [inject]. *)
  mi_no_overlap {injperm: InjectPerm}:
-   forall f m1 m2,
-   inject f m1 m2 ->
+   forall f g m1 m2,
+   inject f g m1 m2 ->
    meminj_no_overlap f m1;
 
  mi_delta_pos {injperm: InjectPerm}:
-   forall f m1 m2 b1 b2 delta,
-     inject f m1 m2 ->
+   forall f g m1 m2 b1 b2 delta,
+     inject f g m1 m2 ->
      f b1 = Some (b2, delta) ->
      delta >= 0;
 
  valid_block_inject_1 {injperm: InjectPerm}:
-  forall f m1 m2 b1 b2 delta,
+  forall f g m1 m2 b1 b2 delta,
   f b1 = Some(b2, delta) ->
-  inject f m1 m2 ->
+  inject f g m1 m2 ->
   valid_block m1 b1;
 
  valid_block_inject_2 {injperm: InjectPerm}:
-  forall f m1 m2 b1 b2 delta,
+  forall f g m1 m2 b1 b2 delta,
   f b1 = Some(b2, delta) ->
-  inject f m1 m2 ->
+  inject f g m1 m2 ->
   valid_block m2 b2;
 
  perm_inject {injperm: InjectPerm}:
-  forall f m1 m2 b1 b2 delta ofs k p,
+  forall f g m1 m2 b1 b2 delta ofs k p,
   f b1 = Some(b2, delta) ->
-  inject f m1 m2 ->
+  inject f g m1 m2 ->
   perm m1 b1 ofs k p ->
   inject_perm_condition p ->
   perm m2 b2 (ofs + delta) k p;
 
  range_perm_inject {injperm: InjectPerm}:
-  forall f m1 m2 b1 b2 delta lo hi k p,
+  forall f g m1 m2 b1 b2 delta lo hi k p,
   f b1 = Some(b2, delta) ->
-  inject f m1 m2 ->
+  inject f g m1 m2 ->
   range_perm m1 b1 lo hi k p ->
   inject_perm_condition p ->
   range_perm m2 b2 (lo + delta) (hi + delta) k p;
 
  valid_access_inject {injperm: InjectPerm}:
-  forall f m1 m2 chunk b1 ofs b2 delta p,
+  forall f g m1 m2 chunk b1 ofs b2 delta p,
   f b1 = Some(b2, delta) ->
-  inject f m1 m2 ->
+  inject f g m1 m2 ->
   valid_access m1 chunk b1 ofs p ->
   inject_perm_condition p ->
   valid_access m2 chunk b2 (ofs + delta) p;
 
  valid_pointer_inject {injperm: InjectPerm}:
-  forall f m1 m2 b1 ofs b2 delta,
+  forall f g m1 m2 b1 ofs b2 delta,
   f b1 = Some(b2, delta) ->
-  inject f m1 m2 ->
+  inject f g m1 m2 ->
   valid_pointer m1 b1 ofs = true ->
   valid_pointer m2 b2 (ofs + delta) = true;
 
  weak_valid_pointer_inject {injperm: InjectPerm}:
-  forall f m1 m2 b1 ofs b2 delta,
+  forall f g m1 m2 b1 ofs b2 delta,
   f b1 = Some(b2, delta) ->
-  inject f m1 m2 ->
+  inject f g m1 m2 ->
   weak_valid_pointer m1 b1 ofs = true ->
   weak_valid_pointer m2 b2 (ofs + delta) = true;
 
  address_inject {injperm: InjectPerm}:
-  forall f m1 m2 b1 ofs1 b2 delta p,
-  inject f m1 m2 ->
+  forall f g m1 m2 b1 ofs1 b2 delta p,
+  inject f g m1 m2 ->
   perm m1 b1 (Ptrofs.unsigned ofs1) Cur p ->
   f b1 = Some (b2, delta) ->
   Ptrofs.unsigned (Ptrofs.add ofs1 (Ptrofs.repr delta)) = Ptrofs.unsigned ofs1 + delta;
 
  (** The following is needed by Separation, to prove storev_parallel_rule *)
  address_inject' {injperm: InjectPerm}:
-  forall f m1 m2 chunk b1 ofs1 b2 delta,
-  inject f m1 m2 ->
+  forall f g m1 m2 chunk b1 ofs1 b2 delta,
+  inject f g m1 m2 ->
   valid_access m1 chunk b1 (Ptrofs.unsigned ofs1) Nonempty ->
   f b1 = Some (b2, delta) ->
   Ptrofs.unsigned (Ptrofs.add ofs1 (Ptrofs.repr delta)) = Ptrofs.unsigned ofs1 + delta;
 
  valid_pointer_inject_no_overflow {injperm: InjectPerm}:
-  forall f m1 m2 b ofs b' delta,
-  inject f m1 m2 ->
+  forall f g m1 m2 b ofs b' delta,
+  inject f g m1 m2 ->
   valid_pointer m1 b (Ptrofs.unsigned ofs) = true ->
   f b = Some(b', delta) ->
   0 <= Ptrofs.unsigned ofs + Ptrofs.unsigned (Ptrofs.repr delta) <= Ptrofs.max_unsigned;
 
  weak_valid_pointer_inject_no_overflow {injperm: InjectPerm}:
-  forall f m1 m2 b ofs b' delta,
-  inject f m1 m2 ->
+  forall f g m1 m2 b ofs b' delta,
+  inject f g m1 m2 ->
   weak_valid_pointer m1 b (Ptrofs.unsigned ofs) = true ->
   f b = Some(b', delta) ->
   0 <= Ptrofs.unsigned ofs + Ptrofs.unsigned (Ptrofs.repr delta) <= Ptrofs.max_unsigned;
 
  valid_pointer_inject_val {injperm: InjectPerm}:
-  forall f m1 m2 b ofs b' ofs',
-  inject f m1 m2 ->
+  forall f g m1 m2 b ofs b' ofs',
+  inject f g m1 m2 ->
   valid_pointer m1 b (Ptrofs.unsigned ofs) = true ->
   Val.inject f (Vptr b ofs) (Vptr b' ofs') ->
   valid_pointer m2 b' (Ptrofs.unsigned ofs') = true;
 
  weak_valid_pointer_inject_val {injperm: InjectPerm}:
-  forall f m1 m2 b ofs b' ofs',
-  inject f m1 m2 ->
+  forall f g m1 m2 b ofs b' ofs',
+  inject f g m1 m2 ->
   weak_valid_pointer m1 b (Ptrofs.unsigned ofs) = true ->
   Val.inject f (Vptr b ofs) (Vptr b' ofs') ->
   weak_valid_pointer m2 b' (Ptrofs.unsigned ofs') = true;
 
  inject_no_overlap {injperm: InjectPerm}:
-  forall f m1 m2 b1 b2 b1' b2' delta1 delta2 ofs1 ofs2,
-  inject f m1 m2 ->
+  forall f g m1 m2 b1 b2 b1' b2' delta1 delta2 ofs1 ofs2,
+  inject f g m1 m2 ->
   b1 <> b2 ->
   f b1 = Some (b1', delta1) ->
   f b2 = Some (b2', delta2) ->
@@ -1219,8 +1218,8 @@ Class MemoryModel mem `{memory_model_ops: MemoryModelOps mem}
   b1' <> b2' \/ ofs1 + delta1 <> ofs2 + delta2;
 
  different_pointers_inject {injperm: InjectPerm}:
-  forall f m m' b1 ofs1 b2 ofs2 b1' delta1 b2' delta2,
-  inject f m m' ->
+  forall f g m m' b1 ofs1 b2 ofs2 b1' delta1 b2' delta2,
+  inject f g m m' ->
   b1 <> b2 ->
   valid_pointer m b1 (Ptrofs.unsigned ofs1) = true ->
   valid_pointer m b2 (Ptrofs.unsigned ofs2) = true ->
@@ -1231,8 +1230,8 @@ Class MemoryModel mem `{memory_model_ops: MemoryModelOps mem}
   Ptrofs.unsigned (Ptrofs.add ofs2 (Ptrofs.repr delta2));
 
  disjoint_or_equal_inject {injperm: InjectPerm}:
-  forall f m m' b1 b1' delta1 b2 b2' delta2 ofs1 ofs2 sz,
-  inject f m m' ->
+  forall f g m m' b1 b1' delta1 b2 b2' delta2 ofs1 ofs2 sz,
+  inject f g m m' ->
   f b1 = Some(b1', delta1) ->
   f b2 = Some(b2', delta2) ->
   range_perm m b1 ofs1 (ofs1 + sz) Max Nonempty ->
@@ -1244,8 +1243,8 @@ Class MemoryModel mem `{memory_model_ops: MemoryModelOps mem}
              \/ ofs2 + delta2 + sz <= ofs1 + delta1;
 
  aligned_area_inject {injperm: InjectPerm}:
-  forall f m m' b ofs al sz b' delta,
-  inject f m m' ->
+  forall f g m m' b ofs al sz b' delta,
+  inject f g m m' ->
   al = 1 \/ al = 2 \/ al = 4 \/ al = 8 -> sz > 0 ->
   (al | sz) ->
   range_perm m b ofs (ofs + sz) Cur Nonempty ->
@@ -1254,116 +1253,116 @@ Class MemoryModel mem `{memory_model_ops: MemoryModelOps mem}
   (al | ofs + delta);
 
  load_inject {injperm: InjectPerm}:
-  forall f m1 m2 chunk b1 ofs b2 delta v1,
-  inject f m1 m2 ->
+  forall f g m1 m2 chunk b1 ofs b2 delta v1,
+  inject f g m1 m2 ->
   load chunk m1 b1 ofs = Some v1 ->
   f b1 = Some (b2, delta) ->
   exists v2, load chunk m2 b2 (ofs + delta) = Some v2 /\ Val.inject f v1 v2;
 
  loadv_inject {injperm: InjectPerm}:
-  forall f m1 m2 chunk a1 a2 v1,
-  inject f m1 m2 ->
+  forall f g m1 m2 chunk a1 a2 v1,
+  inject f g m1 m2 ->
   loadv chunk m1 a1 = Some v1 ->
   Val.inject f a1 a2 ->
   exists v2, loadv chunk m2 a2 = Some v2 /\ Val.inject f v1 v2;
 
  loadbytes_inject {injperm: InjectPerm}:
-  forall f m1 m2 b1 ofs len b2 delta bytes1,
-  inject f m1 m2 ->
+  forall f g m1 m2 b1 ofs len b2 delta bytes1,
+  inject f g m1 m2 ->
   loadbytes m1 b1 ofs len = Some bytes1 ->
   f b1 = Some (b2, delta) ->
   exists bytes2, loadbytes m2 b2 (ofs + delta) len = Some bytes2
               /\ list_forall2 (memval_inject f) bytes1 bytes2;
 
  store_mapped_inject {injperm: InjectPerm}:
-  forall f chunk m1 b1 ofs v1 n1 m2 b2 delta v2,
-  inject f m1 m2 ->
+  forall f g chunk m1 b1 ofs v1 n1 m2 b2 delta v2,
+  inject f g m1 m2 ->
   store chunk m1 b1 ofs v1 = Some n1 ->
   f b1 = Some (b2, delta) ->
   Val.inject f v1 v2 ->
   exists n2,
     store chunk m2 b2 (ofs + delta) v2 = Some n2
-    /\ inject f n1 n2;
+    /\ inject f g n1 n2;
 
  store_unmapped_inject {injperm: InjectPerm}:
-  forall f chunk m1 b1 ofs v1 n1 m2,
-  inject f m1 m2 ->
+  forall f g chunk m1 b1 ofs v1 n1 m2,
+  inject f g m1 m2 ->
   store chunk m1 b1 ofs v1 = Some n1 ->
   f b1 = None ->
-  inject f n1 m2;
+  inject f g n1 m2;
 
  store_outside_inject {injperm: InjectPerm}:
-  forall f m1 m2 chunk b ofs v m2',
-  inject f m1 m2 ->
+  forall f g m1 m2 chunk b ofs v m2',
+  inject f g m1 m2 ->
   (forall b' delta ofs',
     f b' = Some(b, delta) ->
     perm m1 b' ofs' Cur Readable ->
     ofs <= ofs' + delta < ofs + size_chunk chunk -> False) ->
   store chunk m2 b ofs v = Some m2' ->
-  inject f m1 m2';
+  inject f g m1 m2';
 
  storev_mapped_inject {injperm: InjectPerm}:
-  forall f chunk m1 a1 v1 n1 m2 a2 v2,
-  inject f m1 m2 ->
+  forall f g chunk m1 a1 v1 n1 m2 a2 v2,
+  inject f g m1 m2 ->
   storev chunk m1 a1 v1 = Some n1 ->
   Val.inject f a1 a2 ->
   Val.inject f v1 v2 ->
   exists n2,
-    storev chunk m2 a2 v2 = Some n2 /\ inject f n1 n2;
+    storev chunk m2 a2 v2 = Some n2 /\ inject f g n1 n2;
 
  storebytes_mapped_inject {injperm: InjectPerm}:
-  forall f m1 b1 ofs bytes1 n1 m2 b2 delta bytes2,
-  inject f m1 m2 ->
+  forall f g m1 b1 ofs bytes1 n1 m2 b2 delta bytes2,
+  inject f g m1 m2 ->
   storebytes m1 b1 ofs bytes1 = Some n1 ->
   f b1 = Some (b2, delta) ->
   list_forall2 (memval_inject f) bytes1 bytes2 ->
   exists n2,
     storebytes m2 b2 (ofs + delta) bytes2 = Some n2
-    /\ inject f n1 n2;
+    /\ inject f g n1 n2;
 
  storebytes_unmapped_inject {injperm: InjectPerm}:
-  forall f m1 b1 ofs bytes1 n1 m2,
-  inject f m1 m2 ->
+  forall f g m1 b1 ofs bytes1 n1 m2,
+  inject f g m1 m2 ->
   storebytes m1 b1 ofs bytes1 = Some n1 ->
   f b1 = None ->
-  inject f n1 m2;
+  inject f g n1 m2;
 
  storebytes_outside_inject {injperm: InjectPerm}:
-  forall f m1 m2 b ofs bytes2 m2',
-  inject f m1 m2 ->
+  forall f g m1 m2 b ofs bytes2 m2',
+  inject f g m1 m2 ->
   (forall b' delta ofs',
     f b' = Some(b, delta) ->
     perm m1 b' ofs' Cur Readable ->
     ofs <= ofs' + delta < ofs + Z_of_nat (length bytes2) -> False) ->
   storebytes m2 b ofs bytes2 = Some m2' ->
-  inject f m1 m2';
+  inject f g m1 m2';
 
  storebytes_empty_inject {injperm: InjectPerm}:
-  forall f m1 b1 ofs1 m1' m2 b2 ofs2 m2',
-  inject f m1 m2 ->
+  forall f g m1 b1 ofs1 m1' m2 b2 ofs2 m2',
+  inject f g m1 m2 ->
   storebytes m1 b1 ofs1 nil = Some m1' ->
   storebytes m2 b2 ofs2 nil = Some m2' ->
-  inject f m1' m2';
+  inject f g m1' m2';
 
  alloc_right_inject {injperm: InjectPerm}:
-  forall f m1 m2 lo hi b2 m2',
-  inject f m1 m2 ->
+  forall f g m1 m2 lo hi b2 m2',
+  inject f g m1 m2 ->
   alloc m2 lo hi = (m2', b2) ->
-  inject f m1 m2';
+  inject f g m1 m2';
 
  alloc_left_unmapped_inject {injperm: InjectPerm}:
-  forall f m1 m2 lo hi m1' b1,
-  inject f m1 m2 ->
+  forall f g m1 m2 lo hi m1' b1,
+  inject f g m1 m2 ->
   alloc m1 lo hi = (m1', b1) ->
   exists f',
-     inject f' m1' m2
+     inject f' g m1' m2
   /\ inject_incr f f'
   /\ f' b1 = None
   /\ (forall b, b <> b1 -> f' b = f b);
 
  alloc_left_mapped_inject {injperm: InjectPerm}:
-  forall f m1 m2 lo hi m1' b1 b2 delta,
-  inject f m1 m2 ->
+  forall f g m1 m2 lo hi m1' b1 b2 delta,
+  inject f g m1 m2 ->
   alloc m1 lo hi = (m1', b1) ->
   valid_block m2 b2 ->
   0 <= delta <= Ptrofs.max_unsigned ->
@@ -1374,73 +1373,77 @@ Class MemoryModel mem `{memory_model_ops: MemoryModelOps mem}
    f b = Some (b2, delta') ->
    perm m1 b ofs k p ->
    lo + delta <= ofs + delta' < hi + delta -> False) ->
-  ~ in_frames ( (stack_adt m2)) b2 ->
+  (forall (f2 : frame_adt) (fi : frame_info),
+      In f2 (stack_adt m2) ->
+      in_frame f2 b2 ->
+      frame_adt_info f2 = Some fi ->
+      forall (o : Z) (k : perm_kind) (pp : permission), perm m1' b1 o k pp -> inject_perm_condition pp -> frame_public fi (o + delta)) ->
   exists f',
-     inject f' m1' m2
+     inject f' g m1' m2
   /\ inject_incr f f'
   /\ f' b1 = Some(b2, delta)
   /\ (forall b, b <> b1 -> f' b = f b);
 
  alloc_parallel_inject {injperm: InjectPerm}:
-  forall f m1 m2 lo1 hi1 m1' b1 lo2 hi2,
-  inject f m1 m2 ->
+  forall f g m1 m2 lo1 hi1 m1' b1 lo2 hi2,
+  inject f g m1 m2 ->
   alloc m1 lo1 hi1 = (m1', b1) ->
   lo2 <= lo1 -> hi1 <= hi2 ->
   exists f', exists m2', exists b2,
   alloc m2 lo2 hi2 = (m2', b2)
-  /\ inject f' m1' m2'
+  /\ inject f' g m1' m2'
   /\ inject_incr f f'
   /\ f' b1 = Some(b2, 0)
   /\ (forall b, b <> b1 -> f' b = f b);
 
  free_inject {injperm: InjectPerm}:
-  forall f m1 l m1' m2 b lo hi m2',
-  inject f m1 m2 ->
+  forall f g m1 l m1' m2 b lo hi m2',
+  inject f g m1 m2 ->
   free_list m1 l = Some m1' ->
   free m2 b lo hi = Some m2' ->
   (forall b1 delta ofs k p,
     f b1 = Some(b, delta) -> perm m1 b1 ofs k p -> lo <= ofs + delta < hi ->
     exists lo1, exists hi1, In (b1, lo1, hi1) l /\ lo1 <= ofs < hi1) ->
-  inject f m1' m2';
+  inject f g m1' m2';
 
  free_left_inject {injperm: InjectPerm}:
-  forall f m1 m2 b lo hi m1',
-  inject f m1 m2 ->
+  forall f g m1 m2 b lo hi m1',
+  inject f g m1 m2 ->
   free m1 b lo hi = Some m1' ->
-  inject f m1' m2;
+  inject f g m1' m2;
  free_list_left_inject {injperm: InjectPerm}:
-  forall f m2 l m1 m1',
-  inject f m1 m2 ->
+  forall f g m2 l m1 m1',
+  inject f g m1 m2 ->
   free_list m1 l = Some m1' ->
-  inject f m1' m2;
+  inject f g m1' m2;
 
  free_right_inject {injperm: InjectPerm}:
-  forall f m1 m2 b lo hi m2',
-  inject f m1 m2 ->
+  forall f g m1 m2 b lo hi m2',
+  inject f g m1 m2 ->
   free m2 b lo hi = Some m2' ->
   (forall b1 delta ofs k p,
     f b1 = Some(b, delta) -> perm m1 b1 ofs k p ->
     lo <= ofs + delta < hi -> False) ->
-  inject f m1 m2';
+  inject f g m1 m2';
 
  free_parallel_inject {injperm: InjectPerm}:
-  forall f m1 m2 b lo hi m1' b' delta,
-  inject f m1 m2 ->
+  forall f g m1 m2 b lo hi m1' b' delta,
+  inject f g m1 m2 ->
   free m1 b lo hi = Some m1' ->
   f b = Some(b', delta) ->
   inject_perm_condition Freeable ->
   exists m2',
      free m2 b' (lo + delta) (hi + delta) = Some m2'
-  /\ inject f m1' m2';
+  /\ inject f g m1' m2';
 
  drop_outside_inject {injperm: InjectPerm}:
-  forall f m1 m2 b lo hi p m2',
-    inject f m1 m2 ->
+  forall f g m1 m2 b lo hi p m2',
+    inject f g m1 m2 ->
     drop_perm m2 b lo hi p = Some m2' ->
   (forall b' delta ofs k p,
     f b' = Some(b, delta) ->
     perm m1 b' ofs k p -> lo <= ofs + delta < hi -> False) ->
-  inject f m1 m2';
+  inject f g m1 m2';
 
 (** The following property is needed by ValueDomain, to prove mmatch_inj. *)
 
@@ -1452,23 +1455,23 @@ Class MemoryModel mem `{memory_model_ops: MemoryModelOps mem}
      forall o b' o' q n,
        loadbytes m b o 1 = Some (Fragment (Vptr b' o') q n :: nil) ->
        f b' <> None) ->
-  Mem.inject f m m;
+  Mem.inject f (flat_frameinj (length (stack_adt m))) m m;
 
  inject_stack_adt {injperm: InjectPerm}:
-   forall f m1 m2,
-     inject f m1 m2 ->
-     stack_injection f (perm m1) ( (stack_adt m1)) ( (stack_adt m2));
+   forall f g m1 m2,
+     inject f g m1 m2 ->
+     stack_inject f g (perm m1) ( (stack_adt m1)) ( (stack_adt m2));
 
  extends_stack_adt {injperm: InjectPerm}:
    forall m1 m2,
      extends m1 m2 ->
-     stack_injection inject_id (perm m1) (stack_adt m1) (stack_adt m2);
+     stack_inject inject_id (flat_frameinj (length (stack_adt m1))) (perm m1) (stack_adt m1) (stack_adt m2);
 
 (* Needed by Stackingproof, with Linear2 to Mach,
    to compose extends (in Linear2) and inject. *)
  extends_inject_compose {injperm: InjectPerm}:
-   forall f m1 m2 m3,
-     extends m1 m2 -> inject f m2 m3 -> inject f m1 m3;
+   forall f g m1 m2 m3,
+     extends m1 m2 -> inject f g m2 m3 -> inject f g m1 m3;
 
  (* Needed by EraseArgs. *)
  extends_extends_compose {injperm: InjectPerm}:
@@ -1480,7 +1483,7 @@ Class MemoryModel mem `{memory_model_ops: MemoryModelOps mem}
 
  neutral_inject {injperm: InjectPerm}:
   forall m, inject_neutral (nextblock m) m ->
-  inject (flat_inj (nextblock m)) m m;
+  inject (flat_inj (nextblock m)) (flat_frameinj (length (stack_adt m))) m m;
 
  empty_inject_neutral {injperm: InjectPerm}:
   forall thr, inject_neutral thr empty;
@@ -1601,15 +1604,15 @@ drop_perm_stack_adt {injperm: InjectPerm}:
 minjection. HINT: it can be used only for [strong_unchanged_on], not
 for [unchanged_on]. *)
 
- inject_strong_unchanged_on j m0 m m'  {injperm: InjectPerm}:
-   inject j m0 m ->
+ inject_strong_unchanged_on j g m0 m m'  {injperm: InjectPerm}:
+   inject j g m0 m ->
    strong_unchanged_on
      (fun (b : block) (ofs : Z) =>
         exists (b0 : block) (delta : Z),
           j b0 = Some (b, delta) /\
           perm m0 b0 (ofs - delta) Max Nonempty) m m' ->
    stack_adt m' = stack_adt m ->
-   inject j m0 m';
+   inject j g m0 m';
 
  (* Original operations don't modify the abstract part. *)
  store_no_abstract:
@@ -1633,51 +1636,66 @@ for [unchanged_on]. *)
  (* Properties of record_stack_block *)
 
  record_stack_blocks_inject {injperm: InjectPerm}:
-   forall m1 m1' m2 j fi1 fi2,
-     inject j m1 m2 ->
+   forall m1 m1' m2 j g fi1 fi2,
+     inject j g m1 m2 ->
      frame_inject _ j m1 fi1 fi2 ->
-     (forall (b0 b'0 : block) (delta0 : Z),
-         in_frames (stack_adt m1) b0 -> j b0 = Some (b'0, delta0) ->
-         ~ in_frame fi1 b0 /\ ~ in_frame fi2 b'0) ->
+     (forall b : block, in_frames (stack_adt m2) b -> ~ in_frame fi2 b) ->
      (valid_frame fi2 m2) ->
-     record_stack_blocks m1 fi1 = Some m1' ->
+     (forall b fi, in_frame fi2 b -> frame_adt_info fi2 = Some fi ->
+              forall o k p, perm m2 b o k p -> 0 <= o < frame_size fi) ->
+     (forall (b1 b2 : block) (delta : Z), j b1 = Some (b2, delta) -> in_frame fi1 b1 <-> in_frame fi2 b2) ->
+     frame_adt_size fi1 = frame_adt_size fi2 ->
+     record_stack_blocks m1 fi1 m1' ->
      exists m2',
-       record_stack_blocks m2 fi2 = Some m2' /\
-       inject j m1' m2';
+       record_stack_blocks m2 fi2 m2' /\
+       inject j (fun n => if Nat.eq_dec n 0 then Some O else option_map S (g (pred n))) m1' m2';
 
  record_stack_blocks_extends {injperm: InjectPerm}:
     forall m1 m2 m1' fi,
       extends m1 m2 ->
-      record_stack_blocks m1 fi = Some m1' ->
-      (forall b, in_frame fi b -> ~ in_frames ( (stack_adt m1)) b ) ->
+      record_stack_blocks m1 fi m1' ->
+      (forall b, in_frame fi b -> ~ in_frames ( (stack_adt m2)) b ) ->
+      Forall
+        (fun b : block =>
+           forall (o : Z) (k : perm_kind) (p : permission),
+             perm m2 b o k p -> forall fi0 : frame_info, frame_adt_info fi = Some fi0 -> 0 <= o < frame_size fi0) 
+        (frame_blocks fi) ->
       exists m2',
-        record_stack_blocks m2 fi = Some m2' /\
+        record_stack_blocks m2 fi m2' /\
         extends m1' m2';
 
  record_stack_blocks_mem_unchanged:
    forall bfi,
-     mem_unchanged (fun m1 m2 => record_stack_blocks m1 bfi = Some m2);
+     mem_unchanged (fun m1 m2 => record_stack_blocks m1 bfi m2);
 
  record_stack_blocks_stack_adt:
    forall m fi m',
-     record_stack_blocks m fi = Some m' ->
+     record_stack_blocks m fi m' ->
      stack_adt m' = fi :: stack_adt m;
 
  record_stack_blocks_inject_neutral {injperm: InjectPerm}:
    forall thr m fi m',
      inject_neutral thr m ->
-     record_stack_blocks m fi = Some m' ->
-     Forall (fun b => Plt b thr) (frame_blocks fi) ->
+     record_stack_blocks m fi m' ->
      inject_neutral thr m';
 
  (* Properties of unrecord_stack_block *)
 
- unrecord_stack_block_inject {injperm: InjectPerm}:
-   forall (m1 m1' m2 m2' : mem) (j : meminj),
-     inject j m1 m2 ->
+ unrecord_stack_block_inject_parallel {injperm: InjectPerm}:
+   forall (m1 m1' m2 : mem) (j : meminj) g,
+     inject j g m1 m2 ->
      unrecord_stack_block m1 = Some m1' ->
+     (forall i j, g i = Some j -> (O < i) -> (O < j))%nat ->
      exists m2',
-       unrecord_stack_block m2 = Some m2' /\ inject j m1' m2';
+       unrecord_stack_block m2 = Some m2' /\ inject j (fun n => option_map pred (g (S n))) m1' m2';
+
+ unrecord_stack_block_inject_left {injperm: InjectPerm}:
+   forall (m1 m1' m2 : mem) (j : meminj) g,
+     inject j g m1 m2 ->
+     unrecord_stack_block m1 = Some m1' ->
+     g 1%nat = Some O ->
+     (forall b, is_stack_top (stack_adt m1) b -> forall o k p, ~ perm m1 b o k p) ->
+     inject j (fun n => g (S n)) m1' m2;
 
  unrecord_stack_block_extends {injperm: InjectPerm}:
    forall m1 m2 m1',
@@ -1720,9 +1738,9 @@ for [unchanged_on]. *)
      public_stack_access ( (stack_adt m2)) b lo hi;
 
  public_stack_access_inject {injperm: InjectPerm}:
-   forall f m1 m2 b b' delta lo hi p,
+   forall f g m1 m2 b b' delta lo hi p,
      f b = Some (b', delta) ->
-     inject f m1 m2 ->
+     inject f g m1 m2 ->
      range_perm m1 b lo hi Cur p ->
      public_stack_access ( (stack_adt m1)) b lo hi ->
      public_stack_access ( (stack_adt m2)) b' (lo + delta) (hi + delta);
@@ -1734,19 +1752,19 @@ for [unchanged_on]. *)
      public_stack_access ( (stack_adt m2)) b lo hi;
 
 
- not_in_frames_extends {injperm: InjectPerm}:
-   forall m1 m2 b,
-     extends m1 m2 ->
-     ~ in_frames ( (stack_adt m1)) b ->
-     ~ in_frames ( (stack_adt m2)) b;
+ (* not_in_frames_extends {injperm: InjectPerm}: *)
+ (*   forall m1 m2 b, *)
+ (*     extends m1 m2 -> *)
+ (*     ~ in_frames ( (stack_adt m1)) b -> *)
+ (*     ~ in_frames ( (stack_adt m2)) b; *)
 
 
- not_in_frames_inject {injperm: InjectPerm}:
-   forall f m1 m2 b b' delta,
-     f b = Some (b', delta) ->
-     inject f m1 m2 ->
-     ~ in_frames ( (stack_adt m1)) b ->
-     ~ in_frames ( (stack_adt m2)) b';
+ (* not_in_frames_inject {injperm: InjectPerm}: *)
+ (*   forall f g m1 m2 b b' delta, *)
+ (*     f b = Some (b', delta) -> *)
+ (*     inject f g m1 m2 -> *)
+ (*     ~ in_frames ( (stack_adt m1)) b -> *)
+ (*     ~ in_frames ( (stack_adt m2)) b'; *)
 
  in_frames_valid:
    forall m b,
@@ -1759,8 +1777,8 @@ for [unchanged_on]. *)
      is_stack_top ( (stack_adt m2)) b ;
 
  is_stack_top_inject {injperm: InjectPerm}:
-   forall f m1 m2 b1 b2 delta
-     (MINJ: inject f m1 m2)
+   forall f g m1 m2 b1 b2 delta
+     (MINJ: inject f g m1 m2)
      (FB: f b1 = Some (b2, delta))
      (IST: is_stack_top ( (stack_adt m1)) b1),
      is_stack_top ( (stack_adt m2)) b2 ;
@@ -1904,7 +1922,7 @@ Qed.
 
 Lemma record_stack_block_unchanged_on:
   forall m bfi m' (P: block -> Z -> Prop),
-    record_stack_blocks m bfi = Some m' ->
+    record_stack_blocks m bfi m' ->
     strong_unchanged_on P m m'.
 Proof.
   intros; eapply record_stack_blocks_mem_unchanged; eauto.
@@ -1912,7 +1930,7 @@ Qed.
 
 Lemma record_stack_block_perm:
   forall m bfi m',
-    record_stack_blocks m bfi = Some m' ->
+    record_stack_blocks m bfi m' ->
     forall b' o k p,
       perm m' b' o k p ->
       perm m b' o k p.
@@ -1923,7 +1941,7 @@ Qed.
 
 Lemma record_stack_block_perm'
   : forall m m' bofi,
-    record_stack_blocks m bofi = Some m' ->
+    record_stack_blocks m bofi m' ->
     forall (b' : block) (o : Z) (k : perm_kind) (p : permission),
       perm m b' o k p -> perm m' b' o k p.
 Proof.
@@ -1933,7 +1951,7 @@ Qed.
 
 Lemma record_stack_block_valid:
   forall m bf m',
-    record_stack_blocks m bf = Some m' ->
+    record_stack_blocks m bf m' ->
     forall b', valid_block m b' -> valid_block m' b'.
 Proof.
   unfold valid_block; intros.
@@ -1943,7 +1961,7 @@ Qed.
 
 Lemma record_stack_block_nextblock:
   forall m bf m',
-    record_stack_blocks m bf = Some m' ->
+    record_stack_blocks m bf m' ->
     nextblock m' = nextblock m.
 Proof.
   intros.
@@ -1953,7 +1971,7 @@ Qed.
 
 Lemma record_stack_block_is_stack_top:
   forall m b fi m',
-    record_stack_blocks m fi = Some m' ->
+    record_stack_blocks m fi m' ->
     in_frame fi b ->
     is_stack_top (stack_adt m') b.
 Proof.
